Proof for first direction of safety lifting proof

Hyperproperties.v
@@ -2,7 +2,8 @@ From Coq Require Import Lists.List. Import ListNotations.
 From Coq Require Import Lists.Streams.
 From Coq Require Import Sets.Ensembles.
 From Coq Require Import Sets.Powerset.
-From Coq Require Import Sets.Finite_sets. 
+From Coq Require Import Sets.Finite_sets.
+From Coq Require Import Sets.Constructive_sets.
 
 Module Type StateTypeMod.
   Parameter StateType: Type.
@@ -26,10 +27,18 @@ Definition hyperproperty := Ensemble system.
 Definition PROP := Full_set property.
 Definition HP := Full_set hyperproperty.
 
-Definition satisfies_property (S : system) (P : property) :=
-  Included trace S P.
-Definition satisfies_hyperproperty (S : system) (Hp : hyperproperty) :=
-  In system Hp S.
+Definition satisfies_property (s : system) (P : property) :=
+  Included trace s P.
+Definition satisfies_hyperproperty (s : system) (Hp : hyperproperty) :=
+  In system Hp s.
+
+Lemma Rewrite_Included_satisfies_property : forall (s : system) (P : property),
+  Included trace s P = satisfies_property s P.
+Proof. reflexivity. Qed.
+
+Lemma Rewrite_In_satisfies_hyperproperty : forall (s : system) (Hp : hyperproperty),
+  In system Hp s = satisfies_hyperproperty s Hp.
+Proof. reflexivity. Qed.
 
 Definition lift (P : property) : hyperproperty := Power_set trace P.
 
@@ -52,31 +61,55 @@ Inductive prefix : trace -> subtrace -> Prop :=
 Definition prefix_set
   (traces : Ensemble trace)
   (prefixes : Ensemble subtrace) :=
-  forall (t' : subtrace), In (subtrace) prefixes t' ->
-  (exists (t : trace), In (trace) traces t /\ prefix t t').
+  forall (p : subtrace),
+  In (subtrace) prefixes p -> exists (t: trace), In (trace) traces t /\ prefix t p.
+
+(* Definition Obs :=  Full_set (Ensemble subtrace). *)
+Definition Obs := Ensemble subtrace.
 
 Definition safety_property (p: property) :=
-forall (t:trace), forall (t':trace), exists (m:subtrace), ~ In (trace) p t -> 
-( prefix t m /\ ( prefix t' m -> ~ In (trace) p t')) . 
+  forall (t : trace),
+  ~ In (trace) p t -> exists (m : subtrace), forall (t' : trace), prefix t m
+                      /\ (prefix t' m -> ~ In (trace) p t').
 
+Definition safety_hyperproperty (hp: hyperproperty) :=
+  forall (s : system),
+  ~ In (system) hp s -> exists (m : Obs), forall (s': system), prefix_set s m
+                        /\  (prefix_set s' m -> ~ In (system) hp s').
+
+(* The set of all Safety Properties *)
 Definition SP := { p:property | safety_property p}.
 
-Definition Obs :=  Full_set (Ensemble subtrace).
-
-(* fix this to be systems not properties *)
-Definition safety_hyperproperty (h: hyperproperty) := 
-forall (s:system), ( forall (s':system), (exists (M: Ensemble subtrace), ~ In (system) h s -> 
- In (Ensemble subtrace) Obs M /\ prefix_set s M
-/\  prefix_set s' M -> ~ In (property) h s') ).
-
+(* The set of all Safety Hyperproperties *)
 Definition SHP := { h:hyperproperty | safety_hyperproperty h}.
 
-Lemma lifting_preserves_safety:
-  forall (p:property), safety_property p <-> safety_hyperproperty [[p]].
+Lemma not_included_gives_exists : forall (p : property) (s : system),
+  ~ Included trace s p -> exists t : trace, ~ In trace p t /\ In trace s t.
+Proof. Admitted.
+
+Theorem lifting_preserves_safety:
+  forall (p : property), safety_property p <-> safety_hyperproperty [[p]].
 Proof.
   intros p. split; intros H.
-  - unfold safety_hyperproperty. unfold safety_property in H. intros T. intros T'. admit. 
-  - unfold safety_property. unfold safety_hyperproperty in H. intros t'. intros t.  admit. 
-  Admitted.
+  - intros s H'. rewrite Rewrite_In_satisfies_hyperproperty in *.
+    rewrite <- lifting_preserves_satisfiability in *.
+    unfold satisfies_property in H'. unfold not in *.
+    unfold safety_property in H.
+    apply not_included_gives_exists in H'. destruct H' as [t H'']. destruct H'' as [Hp Hs].
+    specialize (H t). apply H in Hp. destruct Hp as [m Hp'].
+    exists (Singleton subtrace m). intros s'. split.
+    + unfold prefix_set. intros p' H0. apply Singleton_inv in H0. rewrite H0 in *.
+      exists t. split.
+      ++ apply Hs.
+      ++ destruct (Hp' t). apply H1.
+    + intros Hpset. rewrite Rewrite_In_satisfies_hyperproperty.
+      rewrite <- lifting_preserves_satisfiability.
+      unfold satisfies_property. unfold prefix_set in Hpset. destruct (Hpset m).
+      ++ apply In_singleton.
+      ++ intros contra. unfold Included in contra. specialize (contra x). destruct H0 as [H0 H0'].
+         apply contra in H0. specialize (Hp' x). destruct Hp' as [Hp' Hp''].
+         apply Hp'' in H0'. contradiction.
+  - admit.
+Admitted.
 
 End Hyperproperty.
